typing for surface language

Surface/Ty/Structure.lean
@@ -6,7 +6,7 @@ import Surface.Ty.BEq
 open LeanSubst
 
 def Surface.Ty.spine : Ty -> Option (String × List Ty)
-| gt#x => return (x, [])
+| gt`#x => return (x, [])
 | app f a => do
   let (x, sp) <- spine f
   (x, sp ++ [a])
@@ -14,11 +14,11 @@ def Surface.Ty.spine : Ty -> Option (String × List Ty)
 
 def Surface.Ty.apply (t : Ty) : List Ty -> Ty
 | [] => t
-| .cons a tl => (t • a).apply tl
+| .cons a tl => (t `• a).apply tl
 
 def Surface.Ty.arity : Ty -> Nat
 | arrow _ B => B.arity + 1
-| ∀[_] P => P.arity + 1
+| `∀[_] P => P.arity + 1
 | _ => 0
 
 inductive Surface.TeleElem
@@ -38,7 +38,7 @@ def Surface.Telescope.rmap (lf : Endo Ren) (r : Ren) : Telescope -> Telescope
 | .cons (.kind K) te => .cons (.kind K) (rmap lf r te)
 | .cons (.ty A) te => .cons (.ty A[r]) (rmap lf (lf r) te)
 
-instance : RenMap Surface.Telescope where
+instance Surface.instRenMap_Telescope : RenMap Surface.Telescope where
   rmap := Surface.Telescope.rmap
 
 def Surface.Telescope.smap (lf : Endo (Subst Surface.Ty)) (σ : Subst Surface.Ty) : Surface.Telescope -> Surface.Telescope
@@ -46,7 +46,7 @@ def Surface.Telescope.smap (lf : Endo (Subst Surface.Ty)) (σ : Subst Surface.Ty
 | .cons (.kind K) te => .cons (.kind K) (smap lf σ te)
 | .cons (.ty A) te => .cons (.ty A[σ]) (smap lf (lf σ) te)
 
-instance : SubstMap Surface.Telescope Surface.Ty where
+instance Surface.instRenMap_TelescopeTy : SubstMap Surface.Telescope Surface.Ty where
   smap := Surface.Telescope.smap
 
 def Surface.Ty.telescope : Ty -> Telescope  × Ty
@@ -67,10 +67,10 @@ def Surface.Ty.from_telescope : List Surface.TeleElem -> Ty -> Ty
 | .nil , t => t
 | .cons (.ty A) tys, t =>
   let r := t.from_telescope tys
-  A -:> r
+  A `-:> r
 | .cons (.kind K) tys, t =>
   let r := t.from_telescope tys
-  ∀[K] r
+  `∀[K] r
 
 @[simp]
 theorem Surface.Ty.Spine.apply_subst {t : Ty} {sp : List Ty} : (t.apply sp)[σ] = (t[σ]).apply (sp.map (·[σ])) := by
@@ -79,7 +79,7 @@ theorem Surface.Ty.Spine.apply_subst {t : Ty} {sp : List Ty} : (t.apply sp)[σ] 
 
 @[simp]
 theorem Surface.Ty.Spine.app_eq :
-  (f • a).spine = some (x, sp)
+  (f `• a).spine = some (x, sp)
   <-> ∃ sp', sp = sp' ++ [a] ∧ f.spine = some (x, sp')
 := by
   apply Iff.intro <;> intro h
@@ -96,12 +96,12 @@ theorem Surface.Ty.Spine.app_eq :
     rw [Option.bind_eq_some_iff]; apply Exists.intro (x, sp')
     apply And.intro e2; simp
 
-theorem Surface.Ty.Spine.apply_type {t : Ty} : t.apply sp • a = t.apply (sp ++ [a]) := by
+theorem Surface.Ty.Spine.apply_type {t : Ty} : t.apply sp `• a = t.apply (sp ++ [a]) := by
   induction sp generalizing t <;> simp [Surface.Ty.apply]
   case cons hd tl ih => rw [ih]
 
 theorem Surface.Ty.Spine.apply_eq
-  : t.spine = some (x, sp) -> t = (gt#x).apply sp
+  : t.spine = some (x, sp) -> t = (gt`#x).apply sp
 := by
   intro h
   fun_induction Surface.Ty.spine generalizing x sp <;> simp at *
@@ -121,10 +121,10 @@ theorem Surface.Ty.Spine.apply_compose {t : Ty}
   intro h; induction sp2 generalizing t x sp1
   simp [Surface.Ty.apply]; exact h
   case _ a tl ih =>
-  have lem : (t • a).spine = some (x, sp1 ++ [a]) := by simp; exact h
+  have lem : (t `• a).spine = some (x, sp1 ++ [a]) := by simp; exact h
   replace ih := ih lem; simp at ih; exact ih
 
 @[simp]
-theorem Surface.Ty.Spine.apply_eta : ((gt#x).apply sp).spine = some (x, sp) := by
-  have lem := @apply_compose x [] sp gt#x (by simp [Surface.Ty.spine])
+theorem Surface.Ty.Spine.apply_eta : ((gt`#x).apply sp).spine = some (x, sp) := by
+  have lem := @apply_compose x [] sp gt`#x (by simp [Surface.Ty.spine])
   simp at lem; exact lem
