Core/Term/BEq.lean
@@ -1,13 +1,93 @@
-import Surface.Ty
-import Surface.Term.Definition
+import Core.Ty
+import Core.Term.Definition
 
-def Surface.Term.beq : Term -> Term -> Bool
+def Ctor0Variant.beq : Ctor0Variant -> Ctor0Variant -> Bool
+| zero, zero => true
+| refl A, refl B => A == B
+| _, _ => false
+
+instance instBEq_Ctor0Variant : BEq Ctor0Variant where
+  beq := Ctor0Variant.beq
+
+instance instReflBEq_Ctor0Variant : ReflBEq Ctor0Variant where
+  rfl := by
+    intro x; induction x <;> simp [instBEq_Ctor0Variant, Ctor0Variant.beq] at *
+
+instance instLawfulBEq_CtorVariant : LawfulBEq Ctor0Variant where
+  eq_of_beq := by
+    intro x b; induction x <;> simp [instBEq_Ctor0Variant, Ctor0Variant.beq] at *
+    all_goals (induction b <;> simp at *)
+
+def Ctor1Variant.beq : Ctor1Variant -> Ctor1Variant -> Bool
+| sym, sym => true
+| fst, fst => true
+| snd, snd => true
+| appt a, appt b => a == b
+| _, _ => false
+
+instance instBEq_Ctor1Variant : BEq Ctor1Variant where
+  beq := Ctor1Variant.beq
+
+instance instReflBEq_Ctor1Variant : ReflBEq Ctor1Variant where
+  rfl := by
+    intro x; induction x <;> simp [instBEq_Ctor1Variant, Ctor1Variant.beq] at *
+
+instance instLawfulBEq_Ctor1Variant : LawfulBEq Ctor1Variant where
+  eq_of_beq := by
+    intro x b; induction x <;> simp [instBEq_Ctor1Variant, Ctor1Variant.beq] at *
+    all_goals (induction b <;> simp at *)
+
+
+def Ctor2Variant.beq : Ctor2Variant -> Ctor2Variant -> Bool
+| app b1, app b2 => b1 == b2
+| cast, cast => true
+| seq, seq => true
+| appc, appc => true
+| apptc, apptc => true
+| arrowc, arrowc => true
+| choice, choice => true
+| _, _ => false
+
+instance instBEq_Ctor2Variant : BEq Ctor2Variant where
+  beq := Ctor2Variant.beq
+
+
+instance instReflBEq_Ctor2Variant : ReflBEq Ctor2Variant where
+  rfl := by
+    intro x; induction x <;> simp [instBEq_Ctor2Variant, Ctor2Variant.beq] at *
+
+instance instLawfulBEq_Ctor2Variant : LawfulBEq Ctor2Variant where
+  eq_of_beq := by
+    intro x b; induction x <;> simp [instBEq_Ctor2Variant, Ctor2Variant.beq] at *
+    all_goals (induction b <;> simp at *)
+
+def TyBindVariant.beq : TyBindVariant -> TyBindVariant -> Bool
+| lamt, lamt => true
+| allc, allc => true
+| _, _ => false
+
+instance instBEq_TyBindVariant : BEq TyBindVariant where
+  beq := TyBindVariant.beq
+
+instance instReflBEq_TyBindVariant : ReflBEq TyBindVariant where
+  rfl := by
+    intro x; induction x <;> simp [instBEq_TyBindVariant, TyBindVariant.beq] at *
+
+instance instLawfulBEq_TyBindVariant : LawfulBEq TyBindVariant where
+  eq_of_beq := by
+    intro x b; induction x <;> simp [instBEq_TyBindVariant, TyBindVariant.beq] at *
+    all_goals (induction b <;> simp at *)
+
+
+def Term.beq : Term -> Term -> Bool
 | var x, var y => x == y
 | global x, global y => x == y
-| appt a1 b1, appt a2 b2 => beq a1 a2 && b1 == b2
-| app a1 b1, app a2 b2 => beq a1 a2 && beq b1 b2
-| lamt K1 t1, lamt K2 t2 => K1 == K2 && beq t1 t2
+| ctor0 c1, ctor0 c2 => c1 == c2
+| ctor1 c1 a1, ctor1 c2 a2 => c1 == c2 && beq a1 a2
+| ctor2 c1 a1 b1, ctor2 c2 a2 b2 => c1 == c2 && beq a1 a2 && beq b1 b2
+| tbind A1 K1 t1, tbind A2 K2 t2 => A1 == A2 && K1 == K2 && beq t1 t2
 | lam A1 t1, lam A2 t2 => A1 == A2 && beq t1 t2
+| guard a1 b1 c1, guard a2 b2 c2 => beq a1 a2 && beq b1 b2 && beq c1 c2
 | .match (n := n1) a1 b1 c1 d1, .match (n := n2) a2 b2 c2 d2 =>
   if h : n1 = n2 then
     let c : Vec Bool n1 := λ i => beq (c1 i) (c2 (by rw [h] at i; exact i))
@@ -16,14 +96,15 @@ def Surface.Term.beq : Term -> Term -> Bool
   else false
 | _, _ => false
 
-instance Surface.instBEq_Term : BEq Surface.Term where
+instance instBEq_Term : BEq Term where
   beq := Term.beq
 
-instance Surface.instReflBEq_Term : ReflBEq Term where
+instance instReflBEq_Term : ReflBEq Term where
   rfl := by
-    intro a; induction a <;> simp [Surface.instBEq_Term, Surface.Term.beq] at *
+    intro a; induction a <;> simp [instBEq_Term, Term.beq] at *
     all_goals (repeat assumption)
     constructor; assumption; assumption
+    constructor; constructor; assumption; assumption; assumption
     case «match» ih1 ih2 ih3 ih4 =>
     constructor
     · constructor
@@ -32,7 +113,7 @@ instance Surface.instReflBEq_Term : ReflBEq Term where
         case _ n _ _ _ _ =>
         induction n
         case _ => simp
-        case _ n ih v1 v2 =>
+        case _ n ih v1 v2 =>         -- split
           simp;
         -- case _ => rfl
         -- case _ =>
@@ -44,11 +125,17 @@ instance Surface.instReflBEq_Term : ReflBEq Term where
       · sorry
     · assumption
 
-instance Surface.instLawfulBEq_Term : LawfulBEq Term where
+instance instLawfulBEq_Term : LawfulBEq Term where
   eq_of_beq := by
     intro a b; cases a <;> simp [instBEq_Term] at *
     all_goals (induction b <;>
-      simp [Term.beq] at *)
+      simp [instBEq_Ctor0Variant, instBEq_Ctor1Variant, instBEq_Ctor2Variant, Term.beq] at *)
+    case _ => intro e; apply eq_of_beq e
+    case _ =>
+      intro e1 e2;
+      constructor
+      apply eq_of_beq e1
+      sorry
     sorry
     sorry
     sorry
