Surface.lean
@@ -1,1 +1,2 @@
-import Surface.Ty.Definition
+import Surface.Ty
+import Surface.Term
