Surface/Term.lean
@@ -1,3 +1,4 @@
 import Surface.Term.Definition
+import Surface.Term.Structure
 import Surface.Term.BEq
--- import Surface.Term.Substitution
+import Surface.Term.Substitution
