Surface/Term/BEq.lean
@@ -1,0 +1,56 @@
+import Surface.Ty
+import Surface.Term.Definition
+
+def Surface.Term.beq : Term -> Term -> Bool
+| var x, var y => x == y
+| global x, global y => x == y
+| appt a1 b1, appt a2 b2 => beq a1 a2 && b1 == b2
+| app a1 b1, app a2 b2 => beq a1 a2 && beq b1 b2
+| lamt K1 t1, lamt K2 t2 => K1 == K2 && beq t1 t2
+| lam A1 t1, lam A2 t2 => A1 == A2 && beq t1 t2
+| .match (n := n1) a1 b1 c1 d1, .match (n := n2) a2 b2 c2 d2 =>
+  if h : n1 = n2 then
+    let c : Vec Bool n1 := λ i => beq (c1 i) (c2 (by rw [h] at i; exact i))
+    let p : Vec Bool n1 := λ i => beq (b1 i) (b2 (by rw[h] at i; exact i))
+    beq a1 a2 && Vec.fold (·&&·) true c && Vec.fold (·&&·) true p && beq d1 d2
+  else false
+| _, _ => false
+
+instance Surface.instBEq_Term : BEq Surface.Term where
+  beq := Term.beq
+
+instance Surface.instReflBEq_Term : ReflBEq Term where
+  rfl := by
+    intro a; induction a <;> simp [Surface.instBEq_Term, Surface.Term.beq] at *
+    all_goals (repeat assumption)
+    constructor; assumption; assumption
+    case «match» ih1 ih2 ih3 ih4 =>
+    constructor
+    · constructor
+      · constructor; assumption;
+        unfold Vec.fold;
+        case _ n _ _ _ _ =>
+        induction n
+        case _ => simp
+        case _ n ih v1 v2 =>
+          simp;
+        -- case _ => rfl
+        -- case _ =>
+        --   split; case _ h =>
+        --   cases h; simp at *
+        --   constructor
+        --   apply ih3
+          sorry
+      · sorry
+    · assumption
+
+instance Surface.instLawfulBEq_Term : LawfulBEq Term where
+  eq_of_beq := by
+    intro a b; cases a <;> simp [instBEq_Term] at *
+    all_goals (induction b <;>
+      simp [Term.beq] at *)
+    sorry
+    sorry
+    sorry
+    sorry
+    sorry
