Surface/Term/Definition.lean
@@ -19,11 +19,37 @@ prefix:max "g`#" => Surface.Term.global
 
 notation f " `•[" a "]" => Surface.Term.appt f a
 
-notation:70 f " • " a:70 => Surface.Term.app f a
+notation:70 f " `• " a:70 => Surface.Term.app f a
 -- notation f " ∘[" a "]" => Surface.Term.ctor2 (Ctor2Variant.app BaseKind.open) f a
 
 -- bind notation
 notation "Λˢ[" K "]" t => Surface.Term.lamt K t
-notation "`λˢ[" A "]" t => Surface.Term.lam A t
+notation "λˢ[" A "]" t => Surface.Term.lam A t
 
 notation "matchˢ!" => Surface.Term.match
+
+
+protected def Surface.Term.repr (p : Nat) : (a : Term) -> Std.Format
+| .var n => "`#" ++ Nat.repr n
+| .global n => "g`#" ++ n
+| .app t1 t2 =>
+  Repr.addAppParen (Term.repr max_prec t1 ++ " • " ++Term.repr p t2) p
+| .appt t1 t2 =>
+  Repr.addAppParen (Term.repr max_prec t1 ++ " •" ++ Std.Format.sbracket (Ty.repr p t2)) p
+| .lamt K t =>
+  Repr.addAppParen ("Λˢ" ++ Std.Format.sbracket (repr K) ++ " " ++ Term.repr max_prec t) p
+| .lam τ t => Repr.addAppParen ("λˢ" ++ Std.Format.sbracket (repr τ) ++ " " ++ Term.repr max_prec t) p
+| .match (n := n) s pats ts allc =>
+  let ts : Vec Std.Format n := λ i =>
+    let t := ts i
+    let pat := pats i
+    Std.Format.nest 4 <| Std.Format.line ++ Term.repr p pat ++ " => " ++ Term.repr p t
+  let css := Vec.fold (·++·) Std.Format.nil ts
+  Std.Format.nest 4 <| (("match " ++ Term.repr max_prec s ++ " with")
+    ++ css
+    ++ (Std.Format.nest 4 <| Std.Format.line ++ " _ => " ++ Term.repr p allc)
+    )
+
+@[simp]
+instance Surface.instRepr_Term : Repr Term where
+  reprPrec a p := Term.repr p a
