Surface/Term/Structure.lean
@@ -1,0 +1,218 @@
+import LeanSubst
+import Core.Util
+import Surface.Term.Definition
+import Surface.Term.Substitution
+import Surface.Term.BEq
+
+open LeanSubst
+
+inductive Surface.SpineElem : Type where
+| type (x : Surface.Ty)
+| term (x : Surface.Term)
+-- | oterm (x : Surface.Term)
+deriving Repr
+
+@[simp]
+def Surface.SpineElem.rmap (_ : Endo Ren) (r : Ren) : SpineElem -> SpineElem
+| type T => type T[r:Ty]
+| term t => term t[r:Term]
+-- | oterm t => oterm t[r:Term]
+
+instance Surface.instRenMap_SpineElem : RenMap Surface.SpineElem where
+  rmap := Surface.SpineElem.rmap
+
+@[simp]
+def Surface.SpineElem.Ty.smap (_ : Endo (Subst Surface.Ty)) (σ : Subst Surface.Ty) : SpineElem -> SpineElem
+| type T => type T[σ]
+| term t => term t[σ:Ty]
+-- | oterm t => oterm t[σ:Ty]
+
+instance Surface.instSubstMap_SpineElemTy : SubstMap Surface.SpineElem Surface.Ty where
+  smap := Surface.SpineElem.Ty.smap
+
+@[simp]
+theorem Surface.SpineElem.Ty.subst_type : (type T)[σ:Ty] = type T[σ] := by
+  simp [Subst.apply, SubstMap.smap]
+
+@[simp]
+theorem Surface.SpineElem.Ty.subst_term : (term T)[σ:Ty] = term T[σ:_] := by
+  simp [Subst.apply, SubstMap.smap]
+
+-- @[simp]
+-- theorem Surface.SpineElem.Ty.subst_oterm : (oterm T)[σ:Ty] = oterm T[σ:_] := by
+--   simp [Subst.apply, SubstMap.smap]
+
+@[simp]
+def Surface.SpineElem.Term.smap (_ : Endo (Subst Term)) (σ : Subst Surface.Term) : Surface.SpineElem -> Surface.SpineElem
+| type T => type T
+| term t => term t[σ]
+
+instance Surface.instSubstMap_SpineElemTerm : SubstMap Surface.SpineElem Surface.Term where
+  smap := Surface.SpineElem.Term.smap
+
+@[simp]
+theorem Surface.SpineElem.Term.subst_type : (type T)[σ:Term] = type T := by
+  simp [Subst.apply, SubstMap.smap]
+
+@[simp]
+theorem Surface.SpineElem.Term.subst_term : (term T)[σ:Term] = term T[σ:_] := by
+  simp [Subst.apply, SubstMap.smap]
+
+-- @[simp]
+-- theorem Surface.SpineElem.Term.subst_oterm : (oterm T)[σ:Term] = oterm T[σ:_] := by
+--   simp [Subst.apply, SubstMap.smap]
+
+def Surface.SpineElem.beq : Surface.SpineElem -> Surface.SpineElem -> Bool
+| .type A, .type B => A == B
+| .term a, .term b => a == b
+| _, _ => false
+
+-- instance Surface.instBEq_SpineElem : BEq Surface.SpineElem where
+--   beq := Surface.SpineElem.beq
+
+-- instance Surface.instReflBEq_SpineElem : ReflBEq Surface.SpineElem where
+--   rfl := by
+--     intro a; cases a <;> simp [Surface.SpineElem.beq, Surface.instBEq_SpineElem] at *
+
+-- instance instLawfulBEq_SpineElem : LawfulBEq SpineElem where
+--   eq_of_beq := by
+--     intro a b; cases a <;> simp [instBEq_SpineElem, SpineElem.beq] at *
+--     all_goals (cases b <;> simp at *)
+
+def Surface.Term.spine : Term -> Option (String × List SpineElem)
+| .global x => return (x, [])
+| .app f a => do
+  let (x, sp) <- spine f
+  (x, sp ++ [.term a])
+| f `•[a] => do
+  let (x, sp) <- spine f
+  (x, sp ++ [.type a])
+| _ => none
+
+def Surface.Term.apply (t : Term) : List SpineElem -> Term
+| [] => t
+| .cons (.type A) tl => (t `•[A]).apply tl
+| .cons (.term a) tl => (t `• a).apply tl
+
+def Surface.Spine.to_subst : List SpineElem -> IteratedSubst
+| [] => .nil
+| .cons (.term t) tl => .term (su t::+0) (Spine.to_subst tl)
+-- | .cons (.oterm t) tl => .term (su t::+0) (Spine.to_subst tl)
+| .cons (.type t) tl => .type (su t::+0) (Spine.to_subst tl)
+
+@[simp]
+theorem Surface.Spine.apply_subst_type {t : Term} : (t.apply sp)[σ:Ty] = (t[σ:_]).apply (sp.map (·[σ:_])) := by
+  induction sp generalizing t <;> simp [Term.apply]
+  case cons hd tl ih =>
+    cases hd <;> simp [Term.apply]
+    all_goals rw [ih]; simp
+
+@[simp]
+theorem Surface.Spine.apply_subst {t : Term} : (t.apply sp)[σ] = (t[σ]).apply (sp.map (·[σ:Term])) := by
+  induction sp generalizing t <;> simp [Term.apply]
+  case cons hd tl ih =>
+    cases hd <;> simp [Term.apply]
+    all_goals rw [ih]; simp
+
+macro "spine_app_eq_solve" x:term : tactic => `(tactic| {
+  apply Iff.intro <;> intro h
+  case _ =>
+    simp [Surface.Term.spine] at h
+    rw [Option.bind_eq_some_iff] at h
+    rcases h with ⟨q, e1, e2⟩
+    rcases q with ⟨y, sp'⟩; simp at e2
+    rcases e2 with ⟨e2, e3⟩; subst e2 e3
+    rw [e1]; exists sp'
+  case _ =>
+    rcases h with ⟨sp', e1, e2⟩; subst e1
+    simp [Surface.Term.spine]
+    rw [Option.bind_eq_some_iff]; apply Exists.intro ($x, sp')
+    apply And.intro e2; simp
+})
+
+@[simp]
+theorem Surface.Spine.app_closed_eq {f a : Surface.Term} :
+  (f `• a).spine = some (x, sp)
+  <-> ∃ sp', sp = sp' ++ [.term a] ∧ f.spine = some (x, sp')
+:= by spine_app_eq_solve x
+
+-- @[simp]
+-- theorem Spine.app_open_eq {f a : Term} :
+--   (f ∘[a]).spine = some (x, sp)
+--   <-> ∃ sp', sp = sp' ++ [.oterm a] ∧ f.spine = some (x, sp')
+-- := by spine_app_eq_solve x
+
+@[simp]
+theorem Surface.Spine.appt_eq {f : Term} :
+  (f `•[a]).spine = some (x, sp)
+  <-> ∃ sp', sp = sp' ++ [.type a] ∧ f.spine = some (x, sp')
+:= by spine_app_eq_solve x
+
+macro "spine_apply_solve" sp:Lean.Parser.Tactic.elimTarget "," t:term : tactic => `(tactic| {
+  induction $sp generalizing $t <;> simp [Surface.Term.apply]
+  case cons hd tl ih _ =>
+  cases hd <;> simp [Surface.Term.apply]
+  all_goals rw [ih]
+})
+
+theorem Surface.Spine.apply_term {t : Term} : t.apply sp `• a = t.apply (sp ++ [.term a]) := by
+  spine_apply_solve sp, t
+
+-- theorem Surface.Spine.apply_oterm {t : Term} : t.apply sp ∘[a] = t.apply (sp ++ [.oterm a]) := by
+--   spine_apply_solve sp, t
+
+theorem Surface.Spine.apply_type {t : Term} : t.apply sp `•[a] = t.apply (sp ++ [.type a]) := by
+  spine_apply_solve sp, t
+
+macro "spine_apply_eq_case_solve"
+  h:term ","
+  ih:term ","
+  ap:Lean.Parser.Tactic.rwRule : tactic =>
+`(tactic| {
+  replace h := $h
+  rw [Option.bind_eq_some_iff] at h
+  rcases h with ⟨q, e1, e2⟩
+  rcases q with ⟨y, sp'⟩; simp at e2
+  rcases e2 with ⟨e2, e3⟩; subst e2 e3
+  replace ih := $ih e1
+  rw [ih, $ap]
+})
+
+theorem Surface.Spine.apply_eq
+  : t.spine = some (x, sp) -> t = (g`#x).apply sp
+:= by
+  intro h
+  fun_induction Term.spine generalizing x sp <;> simp at *
+  case _ y =>
+    rcases h with ⟨e1, e2⟩; subst e1 e2
+    simp [Term.apply]
+  case _ ih => spine_apply_eq_case_solve h, ih, apply_term
+--  case _ ih => spine_apply_eq_case_solve h, ih, apply_oterm
+  case _ ih => spine_apply_eq_case_solve h, ih, apply_type
+
+theorem Surface.Spine.apply_compose {t : Surface.Term}
+  : t.spine = some (x, sp1) -> (t.apply sp2).spine = some (x, sp1 ++ sp2)
+:= by
+  intro h; induction sp2 generalizing t x sp1
+  simp [Term.apply]; exact h
+  case _ hd tl ih =>
+  cases hd <;> simp [Term.apply] at *
+  case _ T =>
+    have lem : (t `•[T]).spine = some (x, sp1 ++ [.type T]) := by simp; exact h
+    replace ih := ih lem; simp at ih; exact ih
+  case _ a =>
+    have lem : (t `• a).spine = some (x, sp1 ++ [.term a]) := by simp; exact h
+    replace ih := ih lem; simp at ih; exact ih
+  -- case _ a =>
+  --   have lem : (t ∘[a]).spine = some (x, sp1 ++ [.oterm a]) := by simp; exact h
+  --   replace ih := ih lem; simp at ih; exact ih
+
+@[simp]
+theorem Surface.Spine.apply_eta : ((g`#x).apply sp).spine = some (x, sp) := by
+  have lem := @apply_compose x [] sp g`#x (by simp [Term.spine])
+  simp at lem; exact lem
+
+theorem Surface.Spine.apply_spine_compose {t : Term}:
+  t.apply (s1 ++ s2) = (t.apply s1).apply s2 := by
+induction t, s1 using Term.apply.induct generalizing s2 <;> simp [Term.apply] at *
+all_goals (case _ ih => apply ih)
