Surface/Term/Substitution.lean
@@ -23,7 +23,7 @@ theorem Surface.Term.from_acton_re {n} : from_action (re n) = `#n := by simp [fr
 @[simp]
 theorem Surface.Term.from_action_su {t} : from_action (su t) = t := by simp [from_action]
 
-instance : Coe (Subst.Action Surface.Term) Surface.Term where
+instance Surface.instCoe_ActionTermTerm : Coe (Subst.Action Surface.Term) Surface.Term where
   coe := Surface.Term.from_action
 
 @[simp]
@@ -36,7 +36,7 @@ def Surface.Term.rmap (lf : Endo Ren) (r : Ren) : Surface.Term -> Surface.Term
 | appt t1 t2 => appt (rmap lf r t1) t2
 | .match t1 t2 t3 t4 => .match (rmap lf r t1) (λ i => rmap lf r (t2 i)) (λ i => rmap lf r (t3 i)) (rmap lf r t4)
 
-instance : RenMap Surface.Term where
+instance Surface.instRenMap_Term : RenMap Surface.Term where
   rmap := Surface.Term.rmap
 
 @[simp]
@@ -49,7 +49,7 @@ def Surface.Term.Ty.smap (lf : Endo (Subst Surface.Ty)) (σ : Subst Surface.Ty) 
 | lam A t => lam A[σ:_] (smap lf σ t)
 | .match t1 t2 t3 t4  => .match (smap lf σ t1) (λ i => smap lf σ (t2 i)) (λ i => smap lf σ (t3 i)) (smap lf σ t4)
 
-instance : SubstMap Surface.Term Surface.Ty where
+instance Surface.instSubstMap_TermTy : SubstMap Surface.Term Surface.Ty where
   smap := Surface.Term.Ty.smap
 
 @[simp]
@@ -62,7 +62,7 @@ def Surface.Term.smap (lf : Endo (Subst Term)) (σ : Subst Term) : Term -> Term
 | lam A t => lam A (smap lf (lf σ) t)
 | .match t1 t2 t3 t4 => .match (smap lf σ t1) (λ i => smap lf σ (t2 i)) (λ i => smap lf σ (t3 i)) (smap lf σ t4)
 
-instance : SubstMap Surface.Term Surface.Term where
+instance Surface.instSubstMap_TermTerm : SubstMap Surface.Term Surface.Term where
   smap := Surface.Term.smap
 
 @[simp]
@@ -136,7 +136,7 @@ theorem Surface.Term.Ty.apply_id {t : Surface.Term} : t[+0:Surface.Ty] = t := by
   induction t
   all_goals (simp at * <;> try simp [*])
 
-instance : SubstMapId Surface.Term Surface.Ty where
+instance Surface.instSubstMapId_Ty_TermTy : SubstMapId Surface.Term Surface.Ty where
   apply_id := Surface.Term.Ty.apply_id
 
 @[simp]
@@ -152,7 +152,7 @@ theorem Surface.Term.apply_stable (r : Ren) (σ : Subst Term)
 := by subst_solve_stable Term, r, σ
 
 
-instance : SubstMapStable Surface.Term where
+instance Surface.instSubstMapStable_Term : SubstMapStable Surface.Term where
   apply_stable := Surface.Term.apply_stable
 
 theorem Surface.Term.apply_ren_commute {s : Surface.Term} (r : Ren) (τ : Subst Surface.Ty)
@@ -165,31 +165,31 @@ theorem Surface.Term.apply_ren_commute {s : Surface.Term} (r : Ren) (τ : Subst 
     rw [Ren.to_lift (S := Surface.Term)] at ih; simp at ih
     apply ih
 
-instance : SubstMapRenCommute Surface.Term Surface.Ty where
+instance Surface.instSubstMapRenCommute_Term : SubstMapRenCommute Surface.Term Surface.Ty where
   apply_ren_commute := Surface.Term.apply_ren_commute
 
 theorem Surface.Term.Ty.apply_compose {s : Term} {σ τ : Subst Ty} : s[σ:Ty][τ:_] = s[σ ∘ τ:_] := by
   subst_solve_compose Surface.Ty, s, σ, τ
 
-instance : SubstMapCompose Surface.Term Surface.Ty where
+instance Surface.instSubstMapCompose_TermTy : SubstMapCompose Surface.Term Surface.Ty where
   apply_compose := Surface.Term.Ty.apply_compose
 
 theorem Surface.Term.apply_hcompose {s : Surface.Term} {σ : Subst Surface.Term} {τ : Subst Surface.Ty}
   : s[σ][τ:_] = s[τ:_][σ ◾ τ]
 := by subst_solve_hcompose Surface.Term, Surface.Ty, s, σ, τ
 
-instance : SubstMapHetCompose Surface.Term Surface.Ty where
+instance Surface.instSubstMapHetCompose_TermTy : SubstMapHetCompose Surface.Term Surface.Ty where
   apply_hcompose := Surface.Term.apply_hcompose
 
 theorem Surface.Term.apply_id {t : Term} : t[+0] = t := by subst_solve_id Term, Ty, t
 
-instance : SubstMapId Surface.Term Surface.Term where
+instance Surface.instSubstMapId_TermTy : SubstMapId Surface.Term Surface.Term where
   apply_id := Surface.Term.apply_id
 
 theorem Surface.Term.apply_compose {s : Surface.Term} {σ τ : Subst Term} : s[σ][τ] = s[σ ∘ τ] := by
   subst_solve_compose Term, s, σ, τ
 
-instance : SubstMapCompose Surface.Term Surface.Term where
+instance Surface.instSubstMapCompose_TermTerm : SubstMapCompose Surface.Term Surface.Term where
   apply_compose := Surface.Term.apply_compose
 
 inductive Surface.IteratedSubst where
