Surface/Ty.lean
@@ -1,3 +1,4 @@
 import Surface.Ty.Definition
 import Surface.Ty.BEq
 import Surface.Ty.Substitution
+import Surface.Ty.Structure
