Surface/Typing.lean
@@ -2,7 +2,37 @@ import LeanSubst
 import Core.Vec
 
 import Surface.Ty
+import Surface.Term
 import Surface.Global
+
+def Surface.ValidHeadVariable (t : Term) (test : String -> Bool) : Prop :=
+  ∃ x, Term.spine t = some x ∧ test x.fst
+
+def Surface.ValidTyHeadVariable (t : Ty) (test : String -> Bool) : Prop :=
+  ∃ x, Ty.spine t = some x ∧ test x.fst
+
+inductive Surface.StableTypeMatch : List Kind -> Ty -> Ty -> Prop
+| refl :
+  Ty.spine R = some x ->
+  StableTypeMatch Δ R R
+| arrow :
+  StableTypeMatch Δ B R ->
+  StableTypeMatch Δ (A `-:> B) R
+| all :
+  StableTypeMatch (K::Δ) B R[+1] ->
+  StableTypeMatch Δ (`∀[K] B) R
+
+
+inductive Surface.PrefixTypeMatch : List Kind -> Ty -> Ty -> Ty -> Prop
+| refl :
+  Ty.spine B = some x ->
+  PrefixTypeMatch Δ B T T
+| arrow :
+  PrefixTypeMatch Δ B V T ->
+  PrefixTypeMatch Δ (A `-:> B) (A `-:> V) T
+| all :
+  PrefixTypeMatch (K::Δ) B V T[+1] ->
+  PrefixTypeMatch Δ (`∀[K] B) (`∀[K] V) T
 
 
 inductive Surface.Kinding (G : List Surface.Global) : List Surface.Kind -> Surface.Ty -> Surface.Kind -> Prop
@@ -26,3 +56,51 @@ inductive Surface.Kinding (G : List Surface.Global) : List Surface.Kind -> Surfa
 
 
 notation:170 G:170 "&" Δ:170 " ⊢s " A:170 " : " K:170 => Surface.Kinding G Δ A K
+
+inductive Surface.Typing (G : List Surface.Global) :
+  List Surface.Kind -> List Surface.Ty -> Surface.Term -> Surface.Ty -> Prop
+| var :
+  Γ[x]? = some A ->
+  G&Δ ⊢s A : .base b ->
+  Typing G Δ Γ `#x A
+| global :
+  lookup_type G x = some A ->
+  G&Δ ⊢s A : .base b ->
+  Typing G Δ Γ g`#x A
+--------------------------------------------------------------------------------------
+---- Matches
+--------------------------------------------------------------------------------------
+| mtch (CTy : Fin n -> Ty)
+       (PTy : Fin n -> Ty)
+       (pats : Vec Term n)
+       (cs : Vec Term n) :
+  Typing G Δ Γ s R ->
+  ValidTyHeadVariable R (is_data G) ->
+  Typing G Δ Γ c T -> -- catch all term is of type T
+  (∀ i, ValidHeadVariable (pats i) (is_ctor G)) -> -- patterns are of the right shape
+  (∀ i, Typing G Δ Γ (pats i) (PTy i)) -> -- each pattern has a type
+  (∀ i, StableTypeMatch Δ (PTy i) R) -> -- the pattern type has a return type that matches datatype
+  (∀ i, Typing G Δ Γ (cs i) (CTy i)) -> -- each case match has a type
+  (∀ i, PrefixTypeMatch Δ (PTy i) (CTy i) T) -> -- patten type and case type
+  Typing G Δ Γ (matchˢ! s pats cs c) T
+--------------------------------------------------------------------------------------
+---- Terms
+--------------------------------------------------------------------------------------
+| lam :
+  G&Δ ⊢s A : .base b ->
+  Typing G Δ (A::Γ) t B ->
+  Typing G Δ Γ (λˢ[A] t) (A `-:> B)
+| app :
+  G&Δ ⊢s A : .base b ->
+  Typing G Δ Γ f (A `-:> B) ->
+  Typing G Δ Γ a A ->
+  Typing G Δ Γ (f `• a) B
+| lamt :
+  Kinding G Δ (`∀[K]P) `★ ->
+  Typing G (K::Δ) (Γ.map (·[+1])) t P ->
+  Typing G Δ Γ (Λˢ[K] t) (`∀[K] P)
+| appt :
+  Typing G Δ Γ f (`∀[K] P) ->
+  G&Δ ⊢s a : K ->
+  P' = P[.su a :: +0:Surface.Ty] ->
+  Typing G Δ Γ (f `•[a]) P'
